feat: Cryptographic Primitives (#15)

AwsCryptographyPrimitives/runtimes/net/Extern/HMAC.cs
@@ -1,0 +1,59 @@
+// Copyright Amazon.com Inc. or its affiliates. All Rights Reserved.
+// SPDX-License-Identifier: Apache-2.0
+
+using System;
+
+using ibyteseq = Dafny.ISequence<byte>;
+using byteseq = Dafny.Sequence<byte>;
+using _IDigestAlgorithm = Dafny.Aws.Cryptography.Primitives.Types._IDigestAlgorithm;
+using Error_Opaque = Dafny.Aws.Cryptography.Primitives.Types.Error_Opaque;
+
+namespace HMAC {
+
+    public partial class HMac {
+
+        private Org.BouncyCastle.Crypto.Macs.HMac hmac;
+
+        public HMac(_IDigestAlgorithm digest) {
+            Org.BouncyCastle.Crypto.IDigest bouncyCastleDigest;
+            if (digest.is_SHA__1) {
+                bouncyCastleDigest = new Org.BouncyCastle.Crypto.Digests.Sha1Digest();
+            } else if(digest.is_SHA__256) {
+                bouncyCastleDigest = new Org.BouncyCastle.Crypto.Digests.Sha256Digest();
+            } else if(digest.is_SHA__384) {
+                bouncyCastleDigest = new Org.BouncyCastle.Crypto.Digests.Sha384Digest();
+            } else if(digest.is_SHA__512) {
+                bouncyCastleDigest = new Org.BouncyCastle.Crypto.Digests.Sha512Digest();
+            } else
+            {
+                throw new System.Exception(String.Format("Unsupported digest: {0}", digest.ToString()));
+            }
+            hmac = new Org.BouncyCastle.Crypto.Macs.HMac(bouncyCastleDigest);
+        }
+
+        public void Init(ibyteseq input) {
+            // KeyParameter/ Init should not mutate input, but this is safer than using input.Elements directly
+            byte[] elemCopy = (byte[]) input.Elements.Clone();
+            var keyParams = new Org.BouncyCastle.Crypto.Parameters.KeyParameter(elemCopy);
+            hmac.Init(keyParams);
+            // elemCopy may contain sensitive info; zeroize it to reduce time this lives in memory
+            Array.Clear(elemCopy, 0, elemCopy.Length);
+            elemCopy = null;
+        }
+
+        public void BlockUpdate(ibyteseq input) {
+            // BlockUpdate should not mutate input, but this is safer than using input.Elements directly
+            byte[] elemCopy = (byte[]) input.Elements.Clone();
+            hmac.BlockUpdate(elemCopy, 0, elemCopy.Length);
+            // elemCopy may contain sensitive info; zeroize it to reduce time this lives in memory
+            Array.Clear(elemCopy, 0, elemCopy.Length);
+            elemCopy = null;
+        }
+
+        public ibyteseq GetResult() {
+            byte[] output = new byte[hmac.GetMacSize()];
+            hmac.DoFinal(output, 0);
+            return byteseq.FromArray(output);
+        }
+    }
+}
