AwsCryptographyPrimitives/runtimes/net/Generated/GenerateRSAKeyPairInput.cs
@@ -1,0 +1,20 @@
+// Copyright Amazon.com Inc. or its affiliates. All Rights Reserved.
+// SPDX-License-Identifier: Apache-2.0
+// Do not modify this file. This file is machine generated, and any changes to it will be overwritten.
+using System;
+ using AWS.Cryptography.Primitives; namespace AWS.Cryptography.Primitives {
+ public class GenerateRSAKeyPairInput {
+ private int? _strength ;
+ public int Strength {
+ get { return this._strength.GetValueOrDefault(); }
+ set { this._strength = value; }
+}
+ internal bool IsSetStrength () {
+ return this._strength.HasValue;
+}
+ public void Validate() {
+ if (!IsSetStrength()) throw new System.ArgumentException("Missing value for required property 'Strength'");
+
+}
+}
+}
