AwsCryptographyPrimitives/runtimes/net/Generated/HMacInput.cs
@@ -1,0 +1,38 @@
+// Copyright Amazon.com Inc. or its affiliates. All Rights Reserved.
+// SPDX-License-Identifier: Apache-2.0
+// Do not modify this file. This file is machine generated, and any changes to it will be overwritten.
+using System;
+ using AWS.Cryptography.Primitives; namespace AWS.Cryptography.Primitives {
+ public class HMacInput {
+ private AWS.Cryptography.Primitives.DigestAlgorithm _digestAlgorithm ;
+ private System.IO.MemoryStream _key ;
+ private System.IO.MemoryStream _message ;
+ public AWS.Cryptography.Primitives.DigestAlgorithm DigestAlgorithm {
+ get { return this._digestAlgorithm; }
+ set { this._digestAlgorithm = value; }
+}
+ internal bool IsSetDigestAlgorithm () {
+ return this._digestAlgorithm != null;
+}
+ public System.IO.MemoryStream Key {
+ get { return this._key; }
+ set { this._key = value; }
+}
+ internal bool IsSetKey () {
+ return this._key != null;
+}
+ public System.IO.MemoryStream Message {
+ get { return this._message; }
+ set { this._message = value; }
+}
+ internal bool IsSetMessage () {
+ return this._message != null;
+}
+ public void Validate() {
+ if (!IsSetDigestAlgorithm()) throw new System.ArgumentException("Missing value for required property 'DigestAlgorithm'");
+ if (!IsSetKey()) throw new System.ArgumentException("Missing value for required property 'Key'");
+ if (!IsSetMessage()) throw new System.ArgumentException("Missing value for required property 'Message'");
+
+}
+}
+}
