AwsCryptographyPrimitives/Model/AwsCryptographyPrimitivesTypes.dfy
@@ -1,0 +1,1002 @@
+// Copyright Amazon.com Inc. or its affiliates. All Rights Reserved.
+// SPDX-License-Identifier: Apache-2.0
+// Do not modify this file. This file is machine generated, and any changes to it will be overwritten.
+include "../../src/StandardLibrary/StandardLibrary.dfy"
+ include "../../src/Util/UTF8.dfy"
+ module {:extern "Dafny.Aws.Cryptography.Primitives.Types" } AwsCryptographyPrimitivesTypes
+ {
+ import opened Wrappers
+ import opened StandardLibrary.UInt
+ import opened UTF8
+ // Generic helpers for verification of mock/unit tests.
+ datatype DafnyCallEvent<I, O> = DafnyCallEvent(input: I, output: O)
+ function Last<T>(s: seq<T>): T requires |s| > 0 { s[|s|-1] }
+ 
+ // Begin Generated Types
+ 
+ datatype AES_CBC = | AES_CBC (
+ nameonly keyLength: SymmetricKeyLength ,
+ nameonly tagLength: Uint8Bytes ,
+ nameonly ivLength: Uint8Bits
+ )
+ datatype AES_GCM = | AES_GCM (
+ nameonly keyLength: SymmetricKeyLength ,
+ nameonly tagLength: Uint8Bytes ,
+ nameonly ivLength: Uint8Bits
+ )
+ datatype AESDecryptInput = | AESDecryptInput (
+ nameonly encAlg: AES_GCM ,
+ nameonly key: seq<uint8> ,
+ nameonly cipherTxt: seq<uint8> ,
+ nameonly authTag: seq<uint8> ,
+ nameonly iv: seq<uint8> ,
+ nameonly aad: seq<uint8>
+ )
+ datatype AESEncryptInput = | AESEncryptInput (
+ nameonly encAlg: AES_GCM ,
+ nameonly iv: seq<uint8> ,
+ nameonly key: seq<uint8> ,
+ nameonly msg: seq<uint8> ,
+ nameonly aad: seq<uint8>
+ )
+ datatype AESEncryptOutput = | AESEncryptOutput (
+ nameonly cipherText: seq<uint8> ,
+ nameonly authTag: seq<uint8>
+ )
+ class IAwsCryptographicPrimitivesClientCallHistory {
+ ghost constructor() {
+ GenerateRandomBytes := [];
+ Digest := [];
+ HMac := [];
+ HkdfExtract := [];
+ HkdfExpand := [];
+ Hkdf := [];
+ AESEncrypt := [];
+ AESDecrypt := [];
+ GenerateRSAKeyPair := [];
+ RSADecrypt := [];
+ RSAEncrypt := [];
+ GenerateECDSASignatureKey := [];
+ ECDSASign := [];
+ ECDSAVerify := [];
+}
+ ghost var GenerateRandomBytes: seq<DafnyCallEvent<GenerateRandomBytesInput, Result<seq<uint8>, Error>>>
+ ghost var Digest: seq<DafnyCallEvent<DigestInput, Result<seq<uint8>, Error>>>
+ ghost var HMac: seq<DafnyCallEvent<HMacInput, Result<seq<uint8>, Error>>>
+ ghost var HkdfExtract: seq<DafnyCallEvent<HkdfExtractInput, Result<seq<uint8>, Error>>>
+ ghost var HkdfExpand: seq<DafnyCallEvent<HkdfExpandInput, Result<seq<uint8>, Error>>>
+ ghost var Hkdf: seq<DafnyCallEvent<HkdfInput, Result<seq<uint8>, Error>>>
+ ghost var AESEncrypt: seq<DafnyCallEvent<AESEncryptInput, Result<AESEncryptOutput, Error>>>
+ ghost var AESDecrypt: seq<DafnyCallEvent<AESDecryptInput, Result<seq<uint8>, Error>>>
+ ghost var GenerateRSAKeyPair: seq<DafnyCallEvent<GenerateRSAKeyPairInput, Result<GenerateRSAKeyPairOutput, Error>>>
+ ghost var RSADecrypt: seq<DafnyCallEvent<RSADecryptInput, Result<seq<uint8>, Error>>>
+ ghost var RSAEncrypt: seq<DafnyCallEvent<RSAEncryptInput, Result<seq<uint8>, Error>>>
+ ghost var GenerateECDSASignatureKey: seq<DafnyCallEvent<GenerateECDSASignatureKeyInput, Result<GenerateECDSASignatureKeyOutput, Error>>>
+ ghost var ECDSASign: seq<DafnyCallEvent<ECDSASignInput, Result<seq<uint8>, Error>>>
+ ghost var ECDSAVerify: seq<DafnyCallEvent<ECDSAVerifyInput, Result<bool, Error>>>
+}
+ trait {:termination false} IAwsCryptographicPrimitivesClient
+ {
+ // Helper to define any additional modifies/reads clauses
+ // If your operations need to mutate state add it
+ // in your constructor function:
+ // Modifies := {your, fields, here, History};
+ // If you do not need to mutate anything:
+ // Modifies := {History};
+ ghost const Modifies: set<object>
+ // For an unassigned const field defined in a trait,
+ // Dafny can only assign a value in the constructor.
+ // This means that for Dafny to reason about this value,
+ // it needs some way to know (an invariant),
+ // about the state of the object.
+ // This builds on the Valid/Repr paradigm
+ // To make this kind requires is safe to add
+ // to methods called from unverified code
+ // the predicate MUST NOT take any arguments.
+ // This means that the correctness of this requires
+ // MUST only be evaluated by the class itself.
+ // If you require any additional mutation,
+ // Then you MUST ensure everything you need in ValidState.
+ // You MUST also ensure ValidState in your constructor.
+ predicate ValidState()
+ ensures ValidState() ==> History in Modifies
+  ghost const History: IAwsCryptographicPrimitivesClientCallHistory
+ predicate GenerateRandomBytesEnsuresPublicly(input: GenerateRandomBytesInput, output: Result<seq<uint8>, Error>)
+ // The public method to be called by library consumers
+ method GenerateRandomBytes ( input: GenerateRandomBytesInput )
+ returns (output: Result<seq<uint8>, Error>)
+ requires
+ && ValidState()
+ modifies Modifies ,
+ History`GenerateRandomBytes
+ // Dafny will skip type parameters when generating a default decreases clause.
+ decreases Modifies
+ ensures
+ && ValidState()
+ ensures GenerateRandomBytesEnsuresPublicly(input, output)
+ ensures History.GenerateRandomBytes == old(History.GenerateRandomBytes) + [DafnyCallEvent(input, output)]
+ 
+ predicate DigestEnsuresPublicly(input: DigestInput, output: Result<seq<uint8>, Error>)
+ // The public method to be called by library consumers
+ method Digest ( input: DigestInput )
+ returns (output: Result<seq<uint8>, Error>)
+ requires
+ && ValidState()
+ modifies Modifies ,
+ History`Digest
+ // Dafny will skip type parameters when generating a default decreases clause.
+ decreases Modifies
+ ensures
+ && ValidState()
+ ensures DigestEnsuresPublicly(input, output)
+ ensures History.Digest == old(History.Digest) + [DafnyCallEvent(input, output)]
+ 
+ predicate HMacEnsuresPublicly(input: HMacInput, output: Result<seq<uint8>, Error>)
+ // The public method to be called by library consumers
+ method HMac ( input: HMacInput )
+ returns (output: Result<seq<uint8>, Error>)
+ requires
+ && ValidState()
+ modifies Modifies ,
+ History`HMac
+ // Dafny will skip type parameters when generating a default decreases clause.
+ decreases Modifies
+ ensures
+ && ValidState()
+ ensures HMacEnsuresPublicly(input, output)
+ ensures History.HMac == old(History.HMac) + [DafnyCallEvent(input, output)]
+ 
+ predicate HkdfExtractEnsuresPublicly(input: HkdfExtractInput, output: Result<seq<uint8>, Error>)
+ // The public method to be called by library consumers
+ method HkdfExtract ( input: HkdfExtractInput )
+ returns (output: Result<seq<uint8>, Error>)
+ requires
+ && ValidState()
+ modifies Modifies ,
+ History`HkdfExtract
+ // Dafny will skip type parameters when generating a default decreases clause.
+ decreases Modifies
+ ensures
+ && ValidState()
+ ensures HkdfExtractEnsuresPublicly(input, output)
+ ensures History.HkdfExtract == old(History.HkdfExtract) + [DafnyCallEvent(input, output)]
+ 
+ predicate HkdfExpandEnsuresPublicly(input: HkdfExpandInput, output: Result<seq<uint8>, Error>)
+ // The public method to be called by library consumers
+ method HkdfExpand ( input: HkdfExpandInput )
+ returns (output: Result<seq<uint8>, Error>)
+ requires
+ && ValidState()
+ modifies Modifies ,
+ History`HkdfExpand
+ // Dafny will skip type parameters when generating a default decreases clause.
+ decreases Modifies
+ ensures
+ && ValidState()
+ ensures HkdfExpandEnsuresPublicly(input, output)
+ ensures History.HkdfExpand == old(History.HkdfExpand) + [DafnyCallEvent(input, output)]
+ 
+ predicate HkdfEnsuresPublicly(input: HkdfInput, output: Result<seq<uint8>, Error>)
+ // The public method to be called by library consumers
+ method Hkdf ( input: HkdfInput )
+ returns (output: Result<seq<uint8>, Error>)
+ requires
+ && ValidState()
+ modifies Modifies ,
+ History`Hkdf
+ // Dafny will skip type parameters when generating a default decreases clause.
+ decreases Modifies
+ ensures
+ && ValidState()
+ ensures HkdfEnsuresPublicly(input, output)
+ ensures History.Hkdf == old(History.Hkdf) + [DafnyCallEvent(input, output)]
+ 
+ predicate AESEncryptEnsuresPublicly(input: AESEncryptInput, output: Result<AESEncryptOutput, Error>)
+ // The public method to be called by library consumers
+ method AESEncrypt ( input: AESEncryptInput )
+ returns (output: Result<AESEncryptOutput, Error>)
+ requires
+ && ValidState()
+ modifies Modifies ,
+ History`AESEncrypt
+ // Dafny will skip type parameters when generating a default decreases clause.
+ decreases Modifies
+ ensures
+ && ValidState()
+ ensures AESEncryptEnsuresPublicly(input, output)
+ ensures History.AESEncrypt == old(History.AESEncrypt) + [DafnyCallEvent(input, output)]
+ 
+ predicate AESDecryptEnsuresPublicly(input: AESDecryptInput, output: Result<seq<uint8>, Error>)
+ // The public method to be called by library consumers
+ method AESDecrypt ( input: AESDecryptInput )
+ returns (output: Result<seq<uint8>, Error>)
+ requires
+ && ValidState()
+ modifies Modifies ,
+ History`AESDecrypt
+ // Dafny will skip type parameters when generating a default decreases clause.
+ decreases Modifies
+ ensures
+ && ValidState()
+ ensures AESDecryptEnsuresPublicly(input, output)
+ ensures History.AESDecrypt == old(History.AESDecrypt) + [DafnyCallEvent(input, output)]
+ 
+ predicate GenerateRSAKeyPairEnsuresPublicly(input: GenerateRSAKeyPairInput, output: Result<GenerateRSAKeyPairOutput, Error>)
+ // The public method to be called by library consumers
+ method GenerateRSAKeyPair ( input: GenerateRSAKeyPairInput )
+ returns (output: Result<GenerateRSAKeyPairOutput, Error>)
+ requires
+ && ValidState()
+ modifies Modifies ,
+ History`GenerateRSAKeyPair
+ // Dafny will skip type parameters when generating a default decreases clause.
+ decreases Modifies
+ ensures
+ && ValidState()
+ ensures GenerateRSAKeyPairEnsuresPublicly(input, output)
+ ensures History.GenerateRSAKeyPair == old(History.GenerateRSAKeyPair) + [DafnyCallEvent(input, output)]
+ 
+ predicate RSADecryptEnsuresPublicly(input: RSADecryptInput, output: Result<seq<uint8>, Error>)
+ // The public method to be called by library consumers
+ method RSADecrypt ( input: RSADecryptInput )
+ returns (output: Result<seq<uint8>, Error>)
+ requires
+ && ValidState()
+ modifies Modifies ,
+ History`RSADecrypt
+ // Dafny will skip type parameters when generating a default decreases clause.
+ decreases Modifies
+ ensures
+ && ValidState()
+ ensures RSADecryptEnsuresPublicly(input, output)
+ ensures History.RSADecrypt == old(History.RSADecrypt) + [DafnyCallEvent(input, output)]
+ 
+ predicate RSAEncryptEnsuresPublicly(input: RSAEncryptInput, output: Result<seq<uint8>, Error>)
+ // The public method to be called by library consumers
+ method RSAEncrypt ( input: RSAEncryptInput )
+ returns (output: Result<seq<uint8>, Error>)
+ requires
+ && ValidState()
+ modifies Modifies ,
+ History`RSAEncrypt
+ // Dafny will skip type parameters when generating a default decreases clause.
+ decreases Modifies
+ ensures
+ && ValidState()
+ ensures RSAEncryptEnsuresPublicly(input, output)
+ ensures History.RSAEncrypt == old(History.RSAEncrypt) + [DafnyCallEvent(input, output)]
+ 
+ predicate GenerateECDSASignatureKeyEnsuresPublicly(input: GenerateECDSASignatureKeyInput, output: Result<GenerateECDSASignatureKeyOutput, Error>)
+ // The public method to be called by library consumers
+ method GenerateECDSASignatureKey ( input: GenerateECDSASignatureKeyInput )
+ returns (output: Result<GenerateECDSASignatureKeyOutput, Error>)
+ requires
+ && ValidState()
+ modifies Modifies ,
+ History`GenerateECDSASignatureKey
+ // Dafny will skip type parameters when generating a default decreases clause.
+ decreases Modifies
+ ensures
+ && ValidState()
+ ensures GenerateECDSASignatureKeyEnsuresPublicly(input, output)
+ ensures History.GenerateECDSASignatureKey == old(History.GenerateECDSASignatureKey) + [DafnyCallEvent(input, output)]
+ 
+ predicate ECDSASignEnsuresPublicly(input: ECDSASignInput, output: Result<seq<uint8>, Error>)
+ // The public method to be called by library consumers
+ method ECDSASign ( input: ECDSASignInput )
+ returns (output: Result<seq<uint8>, Error>)
+ requires
+ && ValidState()
+ modifies Modifies ,
+ History`ECDSASign
+ // Dafny will skip type parameters when generating a default decreases clause.
+ decreases Modifies
+ ensures
+ && ValidState()
+ ensures ECDSASignEnsuresPublicly(input, output)
+ ensures History.ECDSASign == old(History.ECDSASign) + [DafnyCallEvent(input, output)]
+ 
+ predicate ECDSAVerifyEnsuresPublicly(input: ECDSAVerifyInput, output: Result<bool, Error>)
+ // The public method to be called by library consumers
+ method ECDSAVerify ( input: ECDSAVerifyInput )
+ returns (output: Result<bool, Error>)
+ requires
+ && ValidState()
+ modifies Modifies ,
+ History`ECDSAVerify
+ // Dafny will skip type parameters when generating a default decreases clause.
+ decreases Modifies
+ ensures
+ && ValidState()
+ ensures ECDSAVerifyEnsuresPublicly(input, output)
+ ensures History.ECDSAVerify == old(History.ECDSAVerify) + [DafnyCallEvent(input, output)]
+ 
+}
+ datatype CryptoConfig = | CryptoConfig (
+ 
+ )
+ datatype DigestAlgorithm =
+	| SHA_512
+	| SHA_384
+	| SHA_256
+	| SHA_1
+ datatype DigestInput = | DigestInput (
+ nameonly digestAlgorithm: DigestAlgorithm ,
+ nameonly message: seq<uint8>
+ )
+ datatype ECDSASignatureAlgorithm =
+	| ECDSA_P384
+	| ECDSA_P256
+ datatype ECDSASignInput = | ECDSASignInput (
+ nameonly signatureAlgorithm: ECDSASignatureAlgorithm ,
+ nameonly signingKey: seq<uint8> ,
+ nameonly message: seq<uint8>
+ )
+ datatype ECDSAVerifyInput = | ECDSAVerifyInput (
+ nameonly signatureAlgorithm: ECDSASignatureAlgorithm ,
+ nameonly verificationKey: seq<uint8> ,
+ nameonly message: seq<uint8> ,
+ nameonly signature: seq<uint8>
+ )
+ datatype GenerateECDSASignatureKeyInput = | GenerateECDSASignatureKeyInput (
+ nameonly signatureAlgorithm: ECDSASignatureAlgorithm
+ )
+ datatype GenerateECDSASignatureKeyOutput = | GenerateECDSASignatureKeyOutput (
+ nameonly signatureAlgorithm: ECDSASignatureAlgorithm ,
+ nameonly verificationKey: seq<uint8> ,
+ nameonly signingKey: seq<uint8>
+ )
+ datatype GenerateRandomBytesInput = | GenerateRandomBytesInput (
+ nameonly length: PositiveInteger
+ )
+ datatype GenerateRSAKeyPairInput = | GenerateRSAKeyPairInput (
+ nameonly strength: RSAStrengthBits
+ )
+ datatype GenerateRSAKeyPairOutput = | GenerateRSAKeyPairOutput (
+ nameonly publicKey: RSAPublicKey ,
+ nameonly privateKey: RSAPrivateKey
+ )
+ datatype HkdfExpandInput = | HkdfExpandInput (
+ nameonly digestAlgorithm: DigestAlgorithm ,
+ nameonly prk: seq<uint8> ,
+ nameonly info: seq<uint8> ,
+ nameonly expectedLength: PositiveInteger
+ )
+ datatype HkdfExtractInput = | HkdfExtractInput (
+ nameonly digestAlgorithm: DigestAlgorithm ,
+ nameonly salt: Option<seq<uint8>> ,
+ nameonly ikm: seq<uint8>
+ )
+ datatype HkdfInput = | HkdfInput (
+ nameonly digestAlgorithm: DigestAlgorithm ,
+ nameonly salt: Option<seq<uint8>> ,
+ nameonly ikm: seq<uint8> ,
+ nameonly info: seq<uint8> ,
+ nameonly expectedLength: PositiveInteger
+ )
+ datatype HMacInput = | HMacInput (
+ nameonly digestAlgorithm: DigestAlgorithm ,
+ nameonly key: seq<uint8> ,
+ nameonly message: seq<uint8>
+ )
+ type PositiveInteger = x: int32 | IsValid_PositiveInteger(x) witness *
+ predicate method IsValid_PositiveInteger(x: int32) {
+ ( 0 <= x  )
+}
+ datatype RSADecryptInput = | RSADecryptInput (
+ nameonly padding: RSAPaddingMode ,
+ nameonly privateKey: seq<uint8> ,
+ nameonly cipherText: seq<uint8>
+ )
+ datatype RSAEncryptInput = | RSAEncryptInput (
+ nameonly padding: RSAPaddingMode ,
+ nameonly publicKey: seq<uint8> ,
+ nameonly plaintext: seq<uint8>
+ )
+ datatype RSAPaddingMode =
+	| PKCS1
+	| OAEP_SHA1
+	| OAEP_SHA256
+	| OAEP_SHA384
+	| OAEP_SHA512
+ datatype RSAPrivateKey = | RSAPrivateKey (
+ nameonly strength: RSAStrengthBits ,
+ nameonly pem: seq<uint8>
+ )
+ datatype RSAPublicKey = | RSAPublicKey (
+ nameonly strength: RSAStrengthBits ,
+ nameonly pem: seq<uint8>
+ )
+ type RSAStrengthBits = x: int32 | IsValid_RSAStrengthBits(x) witness *
+ predicate method IsValid_RSAStrengthBits(x: int32) {
+ ( 81 <= x <= 80000000 )
+}
+ type SymmetricKeyLength = x: int32 | IsValid_SymmetricKeyLength(x) witness *
+ predicate method IsValid_SymmetricKeyLength(x: int32) {
+ ( 1 <= x <= 32 )
+}
+ type Uint8Bits = x: int32 | IsValid_Uint8Bits(x) witness *
+ predicate method IsValid_Uint8Bits(x: int32) {
+ ( 0 <= x <= 255 )
+}
+ type Uint8Bytes = x: int32 | IsValid_Uint8Bytes(x) witness *
+ predicate method IsValid_Uint8Bytes(x: int32) {
+ ( 0 <= x <= 32 )
+}
+ datatype Error =
+ // Local Error structures are listed here
+ | AwsCryptographicPrimitivesError (
+ nameonly message: string
+ )
+ // Any dependent models are listed here
+ 
+ // The Collection error is used to collect several errors together
+ // This is useful when composing OR logic.
+ // Consider the following method:
+ // 
+ // method FN<I, O>(n:I)
+ //   returns (res: Result<O, Types.Error>)
+ //   ensures A(I).Success? ==> res.Success?
+ //   ensures B(I).Success? ==> res.Success?
+ //   ensures A(I).Failure? && B(I).Failure? ==> res.Failure?
+ // 
+ // If either A || B is successful then FN is successful.
+ // And if A && B fail then FN will fail.
+ // But what information should FN transmit back to the caller?
+ // While it may be correct to hide these details from the caller,
+ // this can not be the globally correct option.
+ // Suppose that A and B can be blocked by different ACLs,
+ // and that their representation of I is only eventually consistent.
+ // How can the caller distinguish, at a minimum for logging,
+ // the difference between the four failure modes?
+ // || (!access(A(I)) && !access(B(I)))
+ // || (!exit(A(I)) && !exit(B(I)))
+ // || (!access(A(I)) && !exit(B(I)))
+ // || (!exit(A(I)) && !access(B(I)))
+ | Collection(list: seq<Error>)
+ // The Opaque error, used for native, extern, wrapped or unknown errors
+ | Opaque(obj: object)
+ type OpaqueError = e: Error | e.Opaque? witness *
+}
+ abstract module AbstractAwsCryptographyPrimitivesService
+ {
+ import opened Wrappers
+ import opened StandardLibrary.UInt
+ import opened UTF8
+ import opened Types = AwsCryptographyPrimitivesTypes
+ import Operations : AbstractAwsCryptographyPrimitivesOperations
+ function method DefaultCryptoConfig(): CryptoConfig
+ method AtomicPrimitives(config: CryptoConfig := DefaultCryptoConfig())
+ returns (res: Result<AtomicPrimitivesClient, Error>)
+ ensures res.Success? ==> 
+ && fresh(res.value)
+ && fresh(res.value.Modifies)
+ && fresh(res.value.History)
+ && res.value.ValidState()
+ class AtomicPrimitivesClient extends IAwsCryptographicPrimitivesClient
+ {
+ constructor(config: Operations.InternalConfig)
+ requires Operations.ValidInternalConfig?(config)
+ ensures
+ && ValidState()
+ && fresh(History)
+ && this.config == config
+ const config: Operations.InternalConfig
+ predicate ValidState()
+ ensures ValidState() ==>
+ && Operations.ValidInternalConfig?(config)
+ && History !in Operations.ModifiesInternalConfig(config)
+ && Modifies == Operations.ModifiesInternalConfig(config) + {History}
+ predicate GenerateRandomBytesEnsuresPublicly(input: GenerateRandomBytesInput, output: Result<seq<uint8>, Error>)
+ {Operations.GenerateRandomBytesEnsuresPublicly(input, output)}
+ // The public method to be called by library consumers
+ method GenerateRandomBytes ( input: GenerateRandomBytesInput )
+ returns (output: Result<seq<uint8>, Error>)
+ requires
+ && ValidState()
+ modifies Modifies ,
+ History`GenerateRandomBytes
+ // Dafny will skip type parameters when generating a default decreases clause.
+ decreases Modifies
+ ensures
+ && ValidState()
+ ensures GenerateRandomBytesEnsuresPublicly(input, output)
+ ensures History.GenerateRandomBytes == old(History.GenerateRandomBytes) + [DafnyCallEvent(input, output)]
+ {
+ output := Operations.GenerateRandomBytes(config, input);
+ History.GenerateRandomBytes := History.GenerateRandomBytes + [DafnyCallEvent(input, output)];
+}
+ 
+ predicate DigestEnsuresPublicly(input: DigestInput, output: Result<seq<uint8>, Error>)
+ {Operations.DigestEnsuresPublicly(input, output)}
+ // The public method to be called by library consumers
+ method Digest ( input: DigestInput )
+ returns (output: Result<seq<uint8>, Error>)
+ requires
+ && ValidState()
+ modifies Modifies ,
+ History`Digest
+ // Dafny will skip type parameters when generating a default decreases clause.
+ decreases Modifies
+ ensures
+ && ValidState()
+ ensures DigestEnsuresPublicly(input, output)
+ ensures History.Digest == old(History.Digest) + [DafnyCallEvent(input, output)]
+ {
+ output := Operations.Digest(config, input);
+ History.Digest := History.Digest + [DafnyCallEvent(input, output)];
+}
+ 
+ predicate HMacEnsuresPublicly(input: HMacInput, output: Result<seq<uint8>, Error>)
+ {Operations.HMacEnsuresPublicly(input, output)}
+ // The public method to be called by library consumers
+ method HMac ( input: HMacInput )
+ returns (output: Result<seq<uint8>, Error>)
+ requires
+ && ValidState()
+ modifies Modifies ,
+ History`HMac
+ // Dafny will skip type parameters when generating a default decreases clause.
+ decreases Modifies
+ ensures
+ && ValidState()
+ ensures HMacEnsuresPublicly(input, output)
+ ensures History.HMac == old(History.HMac) + [DafnyCallEvent(input, output)]
+ {
+ output := Operations.HMac(config, input);
+ History.HMac := History.HMac + [DafnyCallEvent(input, output)];
+}
+ 
+ predicate HkdfExtractEnsuresPublicly(input: HkdfExtractInput, output: Result<seq<uint8>, Error>)
+ {Operations.HkdfExtractEnsuresPublicly(input, output)}
+ // The public method to be called by library consumers
+ method HkdfExtract ( input: HkdfExtractInput )
+ returns (output: Result<seq<uint8>, Error>)
+ requires
+ && ValidState()
+ modifies Modifies ,
+ History`HkdfExtract
+ // Dafny will skip type parameters when generating a default decreases clause.
+ decreases Modifies
+ ensures
+ && ValidState()
+ ensures HkdfExtractEnsuresPublicly(input, output)
+ ensures History.HkdfExtract == old(History.HkdfExtract) + [DafnyCallEvent(input, output)]
+ {
+ output := Operations.HkdfExtract(config, input);
+ History.HkdfExtract := History.HkdfExtract + [DafnyCallEvent(input, output)];
+}
+ 
+ predicate HkdfExpandEnsuresPublicly(input: HkdfExpandInput, output: Result<seq<uint8>, Error>)
+ {Operations.HkdfExpandEnsuresPublicly(input, output)}
+ // The public method to be called by library consumers
+ method HkdfExpand ( input: HkdfExpandInput )
+ returns (output: Result<seq<uint8>, Error>)
+ requires
+ && ValidState()
+ modifies Modifies ,
+ History`HkdfExpand
+ // Dafny will skip type parameters when generating a default decreases clause.
+ decreases Modifies
+ ensures
+ && ValidState()
+ ensures HkdfExpandEnsuresPublicly(input, output)
+ ensures History.HkdfExpand == old(History.HkdfExpand) + [DafnyCallEvent(input, output)]
+ {
+ output := Operations.HkdfExpand(config, input);
+ History.HkdfExpand := History.HkdfExpand + [DafnyCallEvent(input, output)];
+}
+ 
+ predicate HkdfEnsuresPublicly(input: HkdfInput, output: Result<seq<uint8>, Error>)
+ {Operations.HkdfEnsuresPublicly(input, output)}
+ // The public method to be called by library consumers
+ method Hkdf ( input: HkdfInput )
+ returns (output: Result<seq<uint8>, Error>)
+ requires
+ && ValidState()
+ modifies Modifies ,
+ History`Hkdf
+ // Dafny will skip type parameters when generating a default decreases clause.
+ decreases Modifies
+ ensures
+ && ValidState()
+ ensures HkdfEnsuresPublicly(input, output)
+ ensures History.Hkdf == old(History.Hkdf) + [DafnyCallEvent(input, output)]
+ {
+ output := Operations.Hkdf(config, input);
+ History.Hkdf := History.Hkdf + [DafnyCallEvent(input, output)];
+}
+ 
+ predicate AESEncryptEnsuresPublicly(input: AESEncryptInput, output: Result<AESEncryptOutput, Error>)
+ {Operations.AESEncryptEnsuresPublicly(input, output)}
+ // The public method to be called by library consumers
+ method AESEncrypt ( input: AESEncryptInput )
+ returns (output: Result<AESEncryptOutput, Error>)
+ requires
+ && ValidState()
+ modifies Modifies ,
+ History`AESEncrypt
+ // Dafny will skip type parameters when generating a default decreases clause.
+ decreases Modifies
+ ensures
+ && ValidState()
+ ensures AESEncryptEnsuresPublicly(input, output)
+ ensures History.AESEncrypt == old(History.AESEncrypt) + [DafnyCallEvent(input, output)]
+ {
+ output := Operations.AESEncrypt(config, input);
+ History.AESEncrypt := History.AESEncrypt + [DafnyCallEvent(input, output)];
+}
+ 
+ predicate AESDecryptEnsuresPublicly(input: AESDecryptInput, output: Result<seq<uint8>, Error>)
+ {Operations.AESDecryptEnsuresPublicly(input, output)}
+ // The public method to be called by library consumers
+ method AESDecrypt ( input: AESDecryptInput )
+ returns (output: Result<seq<uint8>, Error>)
+ requires
+ && ValidState()
+ modifies Modifies ,
+ History`AESDecrypt
+ // Dafny will skip type parameters when generating a default decreases clause.
+ decreases Modifies
+ ensures
+ && ValidState()
+ ensures AESDecryptEnsuresPublicly(input, output)
+ ensures History.AESDecrypt == old(History.AESDecrypt) + [DafnyCallEvent(input, output)]
+ {
+ output := Operations.AESDecrypt(config, input);
+ History.AESDecrypt := History.AESDecrypt + [DafnyCallEvent(input, output)];
+}
+ 
+ predicate GenerateRSAKeyPairEnsuresPublicly(input: GenerateRSAKeyPairInput, output: Result<GenerateRSAKeyPairOutput, Error>)
+ {Operations.GenerateRSAKeyPairEnsuresPublicly(input, output)}
+ // The public method to be called by library consumers
+ method GenerateRSAKeyPair ( input: GenerateRSAKeyPairInput )
+ returns (output: Result<GenerateRSAKeyPairOutput, Error>)
+ requires
+ && ValidState()
+ modifies Modifies ,
+ History`GenerateRSAKeyPair
+ // Dafny will skip type parameters when generating a default decreases clause.
+ decreases Modifies
+ ensures
+ && ValidState()
+ ensures GenerateRSAKeyPairEnsuresPublicly(input, output)
+ ensures History.GenerateRSAKeyPair == old(History.GenerateRSAKeyPair) + [DafnyCallEvent(input, output)]
+ {
+ output := Operations.GenerateRSAKeyPair(config, input);
+ History.GenerateRSAKeyPair := History.GenerateRSAKeyPair + [DafnyCallEvent(input, output)];
+}
+ 
+ predicate RSADecryptEnsuresPublicly(input: RSADecryptInput, output: Result<seq<uint8>, Error>)
+ {Operations.RSADecryptEnsuresPublicly(input, output)}
+ // The public method to be called by library consumers
+ method RSADecrypt ( input: RSADecryptInput )
+ returns (output: Result<seq<uint8>, Error>)
+ requires
+ && ValidState()
+ modifies Modifies ,
+ History`RSADecrypt
+ // Dafny will skip type parameters when generating a default decreases clause.
+ decreases Modifies
+ ensures
+ && ValidState()
+ ensures RSADecryptEnsuresPublicly(input, output)
+ ensures History.RSADecrypt == old(History.RSADecrypt) + [DafnyCallEvent(input, output)]
+ {
+ output := Operations.RSADecrypt(config, input);
+ History.RSADecrypt := History.RSADecrypt + [DafnyCallEvent(input, output)];
+}
+ 
+ predicate RSAEncryptEnsuresPublicly(input: RSAEncryptInput, output: Result<seq<uint8>, Error>)
+ {Operations.RSAEncryptEnsuresPublicly(input, output)}
+ // The public method to be called by library consumers
+ method RSAEncrypt ( input: RSAEncryptInput )
+ returns (output: Result<seq<uint8>, Error>)
+ requires
+ && ValidState()
+ modifies Modifies ,
+ History`RSAEncrypt
+ // Dafny will skip type parameters when generating a default decreases clause.
+ decreases Modifies
+ ensures
+ && ValidState()
+ ensures RSAEncryptEnsuresPublicly(input, output)
+ ensures History.RSAEncrypt == old(History.RSAEncrypt) + [DafnyCallEvent(input, output)]
+ {
+ output := Operations.RSAEncrypt(config, input);
+ History.RSAEncrypt := History.RSAEncrypt + [DafnyCallEvent(input, output)];
+}
+ 
+ predicate GenerateECDSASignatureKeyEnsuresPublicly(input: GenerateECDSASignatureKeyInput, output: Result<GenerateECDSASignatureKeyOutput, Error>)
+ {Operations.GenerateECDSASignatureKeyEnsuresPublicly(input, output)}
+ // The public method to be called by library consumers
+ method GenerateECDSASignatureKey ( input: GenerateECDSASignatureKeyInput )
+ returns (output: Result<GenerateECDSASignatureKeyOutput, Error>)
+ requires
+ && ValidState()
+ modifies Modifies ,
+ History`GenerateECDSASignatureKey
+ // Dafny will skip type parameters when generating a default decreases clause.
+ decreases Modifies
+ ensures
+ && ValidState()
+ ensures GenerateECDSASignatureKeyEnsuresPublicly(input, output)
+ ensures History.GenerateECDSASignatureKey == old(History.GenerateECDSASignatureKey) + [DafnyCallEvent(input, output)]
+ {
+ output := Operations.GenerateECDSASignatureKey(config, input);
+ History.GenerateECDSASignatureKey := History.GenerateECDSASignatureKey + [DafnyCallEvent(input, output)];
+}
+ 
+ predicate ECDSASignEnsuresPublicly(input: ECDSASignInput, output: Result<seq<uint8>, Error>)
+ {Operations.ECDSASignEnsuresPublicly(input, output)}
+ // The public method to be called by library consumers
+ method ECDSASign ( input: ECDSASignInput )
+ returns (output: Result<seq<uint8>, Error>)
+ requires
+ && ValidState()
+ modifies Modifies ,
+ History`ECDSASign
+ // Dafny will skip type parameters when generating a default decreases clause.
+ decreases Modifies
+ ensures
+ && ValidState()
+ ensures ECDSASignEnsuresPublicly(input, output)
+ ensures History.ECDSASign == old(History.ECDSASign) + [DafnyCallEvent(input, output)]
+ {
+ output := Operations.ECDSASign(config, input);
+ History.ECDSASign := History.ECDSASign + [DafnyCallEvent(input, output)];
+}
+ 
+ predicate ECDSAVerifyEnsuresPublicly(input: ECDSAVerifyInput, output: Result<bool, Error>)
+ {Operations.ECDSAVerifyEnsuresPublicly(input, output)}
+ // The public method to be called by library consumers
+ method ECDSAVerify ( input: ECDSAVerifyInput )
+ returns (output: Result<bool, Error>)
+ requires
+ && ValidState()
+ modifies Modifies ,
+ History`ECDSAVerify
+ // Dafny will skip type parameters when generating a default decreases clause.
+ decreases Modifies
+ ensures
+ && ValidState()
+ ensures ECDSAVerifyEnsuresPublicly(input, output)
+ ensures History.ECDSAVerify == old(History.ECDSAVerify) + [DafnyCallEvent(input, output)]
+ {
+ output := Operations.ECDSAVerify(config, input);
+ History.ECDSAVerify := History.ECDSAVerify + [DafnyCallEvent(input, output)];
+}
+ 
+}
+}
+ abstract module AbstractAwsCryptographyPrimitivesOperations {
+ import opened Wrappers
+ import opened StandardLibrary.UInt
+ import opened UTF8
+ import opened Types = AwsCryptographyPrimitivesTypes
+ type InternalConfig
+ predicate ValidInternalConfig?(config: InternalConfig)
+ function ModifiesInternalConfig(config: InternalConfig): set<object>
+ predicate GenerateRandomBytesEnsuresPublicly(input: GenerateRandomBytesInput, output: Result<seq<uint8>, Error>)
+ // The private method to be refined by the library developer
+
+
+ method GenerateRandomBytes ( config: InternalConfig,  input: GenerateRandomBytesInput )
+ returns (output: Result<seq<uint8>, Error>)
+ requires
+ && ValidInternalConfig?(config)
+ modifies ModifiesInternalConfig(config)
+ // Dafny will skip type parameters when generating a default decreases clause.
+ decreases ModifiesInternalConfig(config)
+ ensures
+ && ValidInternalConfig?(config)
+ ensures GenerateRandomBytesEnsuresPublicly(input, output)
+
+
+ predicate DigestEnsuresPublicly(input: DigestInput, output: Result<seq<uint8>, Error>)
+ // The private method to be refined by the library developer
+
+
+ method Digest ( config: InternalConfig,  input: DigestInput )
+ returns (output: Result<seq<uint8>, Error>)
+ requires
+ && ValidInternalConfig?(config)
+ modifies ModifiesInternalConfig(config)
+ // Dafny will skip type parameters when generating a default decreases clause.
+ decreases ModifiesInternalConfig(config)
+ ensures
+ && ValidInternalConfig?(config)
+ ensures DigestEnsuresPublicly(input, output)
+
+
+ predicate HMacEnsuresPublicly(input: HMacInput, output: Result<seq<uint8>, Error>)
+ // The private method to be refined by the library developer
+
+
+ method HMac ( config: InternalConfig,  input: HMacInput )
+ returns (output: Result<seq<uint8>, Error>)
+ requires
+ && ValidInternalConfig?(config)
+ modifies ModifiesInternalConfig(config)
+ // Dafny will skip type parameters when generating a default decreases clause.
+ decreases ModifiesInternalConfig(config)
+ ensures
+ && ValidInternalConfig?(config)
+ ensures HMacEnsuresPublicly(input, output)
+
+
+ predicate HkdfExtractEnsuresPublicly(input: HkdfExtractInput, output: Result<seq<uint8>, Error>)
+ // The private method to be refined by the library developer
+
+
+ method HkdfExtract ( config: InternalConfig,  input: HkdfExtractInput )
+ returns (output: Result<seq<uint8>, Error>)
+ requires
+ && ValidInternalConfig?(config)
+ modifies ModifiesInternalConfig(config)
+ // Dafny will skip type parameters when generating a default decreases clause.
+ decreases ModifiesInternalConfig(config)
+ ensures
+ && ValidInternalConfig?(config)
+ ensures HkdfExtractEnsuresPublicly(input, output)
+
+
+ predicate HkdfExpandEnsuresPublicly(input: HkdfExpandInput, output: Result<seq<uint8>, Error>)
+ // The private method to be refined by the library developer
+
+
+ method HkdfExpand ( config: InternalConfig,  input: HkdfExpandInput )
+ returns (output: Result<seq<uint8>, Error>)
+ requires
+ && ValidInternalConfig?(config)
+ modifies ModifiesInternalConfig(config)
+ // Dafny will skip type parameters when generating a default decreases clause.
+ decreases ModifiesInternalConfig(config)
+ ensures
+ && ValidInternalConfig?(config)
+ ensures HkdfExpandEnsuresPublicly(input, output)
+
+
+ predicate HkdfEnsuresPublicly(input: HkdfInput, output: Result<seq<uint8>, Error>)
+ // The private method to be refined by the library developer
+
+
+ method Hkdf ( config: InternalConfig,  input: HkdfInput )
+ returns (output: Result<seq<uint8>, Error>)
+ requires
+ && ValidInternalConfig?(config)
+ modifies ModifiesInternalConfig(config)
+ // Dafny will skip type parameters when generating a default decreases clause.
+ decreases ModifiesInternalConfig(config)
+ ensures
+ && ValidInternalConfig?(config)
+ ensures HkdfEnsuresPublicly(input, output)
+
+
+ predicate AESEncryptEnsuresPublicly(input: AESEncryptInput, output: Result<AESEncryptOutput, Error>)
+ // The private method to be refined by the library developer
+
+
+ method AESEncrypt ( config: InternalConfig,  input: AESEncryptInput )
+ returns (output: Result<AESEncryptOutput, Error>)
+ requires
+ && ValidInternalConfig?(config)
+ modifies ModifiesInternalConfig(config)
+ // Dafny will skip type parameters when generating a default decreases clause.
+ decreases ModifiesInternalConfig(config)
+ ensures
+ && ValidInternalConfig?(config)
+ ensures AESEncryptEnsuresPublicly(input, output)
+
+
+ predicate AESDecryptEnsuresPublicly(input: AESDecryptInput, output: Result<seq<uint8>, Error>)
+ // The private method to be refined by the library developer
+
+
+ method AESDecrypt ( config: InternalConfig,  input: AESDecryptInput )
+ returns (output: Result<seq<uint8>, Error>)
+ requires
+ && ValidInternalConfig?(config)
+ modifies ModifiesInternalConfig(config)
+ // Dafny will skip type parameters when generating a default decreases clause.
+ decreases ModifiesInternalConfig(config)
+ ensures
+ && ValidInternalConfig?(config)
+ ensures AESDecryptEnsuresPublicly(input, output)
+
+
+ predicate GenerateRSAKeyPairEnsuresPublicly(input: GenerateRSAKeyPairInput, output: Result<GenerateRSAKeyPairOutput, Error>)
+ // The private method to be refined by the library developer
+
+
+ method GenerateRSAKeyPair ( config: InternalConfig,  input: GenerateRSAKeyPairInput )
+ returns (output: Result<GenerateRSAKeyPairOutput, Error>)
+ requires
+ && ValidInternalConfig?(config)
+ modifies ModifiesInternalConfig(config)
+ // Dafny will skip type parameters when generating a default decreases clause.
+ decreases ModifiesInternalConfig(config)
+ ensures
+ && ValidInternalConfig?(config)
+ ensures GenerateRSAKeyPairEnsuresPublicly(input, output)
+
+
+ predicate RSADecryptEnsuresPublicly(input: RSADecryptInput, output: Result<seq<uint8>, Error>)
+ // The private method to be refined by the library developer
+
+
+ method RSADecrypt ( config: InternalConfig,  input: RSADecryptInput )
+ returns (output: Result<seq<uint8>, Error>)
+ requires
+ && ValidInternalConfig?(config)
+ modifies ModifiesInternalConfig(config)
+ // Dafny will skip type parameters when generating a default decreases clause.
+ decreases ModifiesInternalConfig(config)
+ ensures
+ && ValidInternalConfig?(config)
+ ensures RSADecryptEnsuresPublicly(input, output)
+
+
+ predicate RSAEncryptEnsuresPublicly(input: RSAEncryptInput, output: Result<seq<uint8>, Error>)
+ // The private method to be refined by the library developer
+
+
+ method RSAEncrypt ( config: InternalConfig,  input: RSAEncryptInput )
+ returns (output: Result<seq<uint8>, Error>)
+ requires
+ && ValidInternalConfig?(config)
+ modifies ModifiesInternalConfig(config)
+ // Dafny will skip type parameters when generating a default decreases clause.
+ decreases ModifiesInternalConfig(config)
+ ensures
+ && ValidInternalConfig?(config)
+ ensures RSAEncryptEnsuresPublicly(input, output)
+
+
+ predicate GenerateECDSASignatureKeyEnsuresPublicly(input: GenerateECDSASignatureKeyInput, output: Result<GenerateECDSASignatureKeyOutput, Error>)
+ // The private method to be refined by the library developer
+
+
+ method GenerateECDSASignatureKey ( config: InternalConfig,  input: GenerateECDSASignatureKeyInput )
+ returns (output: Result<GenerateECDSASignatureKeyOutput, Error>)
+ requires
+ && ValidInternalConfig?(config)
+ modifies ModifiesInternalConfig(config)
+ // Dafny will skip type parameters when generating a default decreases clause.
+ decreases ModifiesInternalConfig(config)
+ ensures
+ && ValidInternalConfig?(config)
+ ensures GenerateECDSASignatureKeyEnsuresPublicly(input, output)
+
+
+ predicate ECDSASignEnsuresPublicly(input: ECDSASignInput, output: Result<seq<uint8>, Error>)
+ // The private method to be refined by the library developer
+
+
+ method ECDSASign ( config: InternalConfig,  input: ECDSASignInput )
+ returns (output: Result<seq<uint8>, Error>)
+ requires
+ && ValidInternalConfig?(config)
+ modifies ModifiesInternalConfig(config)
+ // Dafny will skip type parameters when generating a default decreases clause.
+ decreases ModifiesInternalConfig(config)
+ ensures
+ && ValidInternalConfig?(config)
+ ensures ECDSASignEnsuresPublicly(input, output)
+
+
+ predicate ECDSAVerifyEnsuresPublicly(input: ECDSAVerifyInput, output: Result<bool, Error>)
+ // The private method to be refined by the library developer
+
+
+ method ECDSAVerify ( config: InternalConfig,  input: ECDSAVerifyInput )
+ returns (output: Result<bool, Error>)
+ requires
+ && ValidInternalConfig?(config)
+ modifies ModifiesInternalConfig(config)
+ // Dafny will skip type parameters when generating a default decreases clause.
+ decreases ModifiesInternalConfig(config)
+ ensures
+ && ValidInternalConfig?(config)
+ ensures ECDSAVerifyEnsuresPublicly(input, output)
+}
