AwsCryptographyPrimitives/src/AwsCryptographyPrimitivesOperations.dfy
@@ -1,0 +1,171 @@
+// Copyright Amazon.com Inc. or its affiliates. All Rights Reserved.
+// SPDX-License-Identifier: Apache-2.0
+
+include "../Model/AwsCryptographyPrimitivesTypes.dfy"
+include "Random.dfy"
+include "WrappedHMAC.dfy"
+include "WrappedHKDF.dfy"
+include "AESEncryption.dfy"
+include "Digest.dfy"
+include "RSAEncryption.dfy"
+include "Signature.dfy"
+
+module AwsCryptographyPrimitivesOperations refines AbstractAwsCryptographyPrimitivesOperations {
+  import Random
+  import AESEncryption
+  import D = Digest
+  import WrappedHMAC
+  import WrappedHKDF
+  import Signature
+  import RSAEncryption
+
+  datatype Config = Config
+  type InternalConfig = Config
+  predicate ValidInternalConfig?(config: InternalConfig)
+  {true}
+  function ModifiesInternalConfig(config: InternalConfig) : set<object>
+  {{}}
+
+  predicate GenerateRandomBytesEnsuresPublicly(input: GenerateRandomBytesInput, output: Result<seq<uint8>, Error>)
+  {
+    output.Success? ==> |output.value| == input.length as int
+  }
+
+  method GenerateRandomBytes ( config: InternalConfig,  input: GenerateRandomBytesInput )
+    returns (output: Result<seq<uint8>, Error>)
+  {
+    output := Random.GenerateBytes(input.length);
+  }
+
+  predicate DigestEnsuresPublicly(input: DigestInput, output: Result<seq<uint8>, Error>)
+  {true}
+
+  method Digest ( config: InternalConfig,  input: DigestInput )
+    returns (output: Result<seq<uint8>, Error>)
+  {
+    output := D.Digest(input);
+  }
+
+  predicate HMacEnsuresPublicly(input: HMacInput, output: Result<seq<uint8>, Error>)
+  {true}
+
+  method HMac ( config: InternalConfig,  input: HMacInput )
+    returns (output: Result<seq<uint8>, Error>)
+  {
+    output := WrappedHMAC.Digest(input);
+  }
+
+  predicate HkdfExtractEnsuresPublicly(input: HkdfExtractInput, output: Result<seq<uint8>, Error>)
+  {true}
+
+  method HkdfExtract ( config: InternalConfig,  input: HkdfExtractInput )
+    returns (output: Result<seq<uint8>, Error>)
+  {
+    output := WrappedHKDF.Extract(input);
+  }
+
+  predicate HkdfExpandEnsuresPublicly(input: HkdfExpandInput, output: Result<seq<uint8>, Error>)
+  {true}
+
+  method HkdfExpand ( config: InternalConfig,  input: HkdfExpandInput )
+    returns (output: Result<seq<uint8>, Error>)
+  {
+    output := WrappedHKDF.Expand(input);
+  }
+
+  predicate HkdfEnsuresPublicly(input: HkdfInput, output: Result<seq<uint8>, Error>)
+  {true}
+
+  method Hkdf ( config: InternalConfig,  input: HkdfInput )
+    returns (output: Result<seq<uint8>, Error>)
+  {
+    output := WrappedHKDF.Hkdf(input);
+  }
+
+  predicate AESEncryptEnsuresPublicly(input: AESEncryptInput, output: Result<AESEncryptOutput, Error>)
+  {
+      && output.Success?
+    ==>
+      && |output.value.cipherText| == |input.msg|
+      && |output.value.authTag| == input.encAlg.tagLength as nat
+  }
+
+  method AESEncrypt ( config: InternalConfig,  input: AESEncryptInput )
+    returns (output: Result<AESEncryptOutput, Error>)
+  {
+    output := AESEncryption.AESEncrypt(input);
+  }
+
+  predicate AESDecryptEnsuresPublicly(input: AESDecryptInput, output: Result<seq<uint8>, Error>)
+  {
+      && output.Success?
+    ==>
+      && |output.value| == |input.cipherTxt|
+  }
+
+  method AESDecrypt ( config: InternalConfig,  input: AESDecryptInput )
+    returns (output: Result<seq<uint8>, Error>)
+  {
+    output := AESEncryption.AESDecrypt(input);
+  }
+
+  predicate GenerateRSAKeyPairEnsuresPublicly(input: GenerateRSAKeyPairInput, output: Result<GenerateRSAKeyPairOutput, Error>)
+  {true}
+
+  method GenerateRSAKeyPair ( config: InternalConfig,  input: GenerateRSAKeyPairInput )
+    returns (output: Result<GenerateRSAKeyPairOutput, Error>)
+  {
+    var publicKey, privateKey := RSAEncryption.GenerateKeyPair(input.strength);
+    output := Success(GenerateRSAKeyPairOutput(publicKey := publicKey, privateKey := privateKey));
+  }
+
+  predicate RSADecryptEnsuresPublicly(input: RSADecryptInput, output: Result<seq<uint8>, Error>)
+  {true}
+
+  method RSADecrypt ( config: InternalConfig,  input: RSADecryptInput )
+    returns (output: Result<seq<uint8>, Error>)
+  {
+    output := RSAEncryption.Decrypt(input);
+  }
+
+  predicate RSAEncryptEnsuresPublicly(input: RSAEncryptInput, output: Result<seq<uint8>, Error>)
+  {true}
+
+  method RSAEncrypt ( config: InternalConfig,  input: RSAEncryptInput )
+    returns (output: Result<seq<uint8>, Error>)
+  {
+    output := RSAEncryption.Encrypt(input);
+  }
+
+  predicate GenerateECDSASignatureKeyEnsuresPublicly(input: GenerateECDSASignatureKeyInput, output: Result<GenerateECDSASignatureKeyOutput, Error>)
+  {true}
+
+  method GenerateECDSASignatureKey ( config: InternalConfig,  input: GenerateECDSASignatureKeyInput )
+    returns (output: Result<GenerateECDSASignatureKeyOutput, Error>)
+  {
+    output := Signature.KeyGen(input);
+  }
+
+  predicate ECDSASignEnsuresPublicly(input: ECDSASignInput, output: Result<seq<uint8>, Error>)
+  {true}
+
+  method ECDSASign ( config: InternalConfig,  input: ECDSASignInput )
+    returns (output: Result<seq<uint8>, Error>)
+  {
+    output := Signature.Sign(input.signatureAlgorithm, input.signingKey, input.message);
+  }
+
+  predicate ECDSAVerifyEnsuresPublicly(input: ECDSAVerifyInput, output: Result<bool, Error>)
+  {true}
+
+  method ECDSAVerify ( config: InternalConfig,  input: ECDSAVerifyInput )
+    returns (output: Result<bool, Error>)
+  {
+    output := Signature.Verify(
+      input.signatureAlgorithm,
+      input.verificationKey,
+      input.message,
+      input.signature
+    );
+  }
+}
