AwsCryptographyPrimitives/src/HKDF/HMAC.dfy
@@ -1,0 +1,51 @@
+// Copyright Amazon.com Inc. or its affiliates. All Rights Reserved.
+// SPDX-License-Identifier: Apache-2.0
+
+include "../../Model/AwsCryptographyPrimitivesTypes.dfy"
+include "../Digest.dfy"
+
+module {:extern "HMAC"} HMAC {
+  import opened StandardLibrary
+  import opened UInt = StandardLibrary.UInt
+  import Types = AwsCryptographyPrimitivesTypes
+  import Digest
+
+  class {:extern "HMac"} HMac {
+
+    // These functions are used to model the extern state
+    // https://github.com/dafny-lang/dafny/wiki/Modeling-External-State-Correctly
+    function {:extern} GetKey(): seq<uint8> reads this
+    function {:extern} GetDigest(): Types.DigestAlgorithm reads this
+    function {:extern} GetInputSoFar(): seq<uint8> reads this
+
+    constructor {:extern} (digest: Types.DigestAlgorithm)
+      ensures this.GetDigest() == digest
+      ensures this.GetInputSoFar() == []
+
+    method {:extern "Init"} Init(key: seq<uint8>)
+      modifies this
+      ensures this.GetKey() == key;
+      ensures this.GetDigest() == old(this.GetDigest())
+      ensures this.GetInputSoFar() == []
+
+    method {:extern "BlockUpdate"} Update(input: seq<uint8>)
+      requires |this.GetKey()| > 0
+      requires |input| < INT32_MAX_LIMIT
+      modifies this
+      ensures this.GetInputSoFar() == old(this.GetInputSoFar()) + input
+      ensures this.GetDigest() == old(this.GetDigest())
+      ensures this.GetKey() == old(this.GetKey())
+
+    method {:extern "GetResult"} GetResult() returns (s: seq<uint8>)
+      requires |this.GetKey()| > 0
+      modifies this
+      ensures |s| == Digest.Length(this.GetDigest())
+      ensures this.GetInputSoFar() == []
+      ensures this.GetDigest() == old(this.GetDigest())
+      ensures this.GetKey() == old(this.GetKey())
+      ensures this.HashSignature(old(this.GetInputSoFar()), s);
+
+    predicate {:axiom} HashSignature(message: seq<uint8>, s: seq<uint8>)
+
+  }
+}
