AwsCryptographyPrimitives/src/RSAEncryption.dfy
@@ -1,0 +1,56 @@
+// Copyright Amazon.com Inc. or its affiliates. All Rights Reserved.
+// SPDX-License-Identifier: Apache-2.0
+
+include "../Model/AwsCryptographyPrimitivesTypes.dfy"
+
+module {:extern "RSAEncryption"} RSAEncryption {
+  import opened Wrappers
+  import opened UInt = StandardLibrary.UInt
+  import Types = AwsCryptographyPrimitivesTypes
+
+  // The smallest ciphertext length is defined using PKCS1, where messageLength <= k - 11 and k represents the strength,
+  // defined as the length in octets (bytes) of the modulus n. This means that the minimum possible strength in bits
+  // can be calculated as: (strength + 7) / 8 - 11 == 0 ==> min strength == 81 in this scenario
+  // (where messageLength == 0). In practice, this number should be much higher (at least 1024 or, better, 2048).
+  // TODO: Determine if we want to enforce a min value of 2048 bits as the min strength (requires updating the spec)
+  // newtype {:nativeType "int", "number"} StrengthBits = x | 81 <= x < (0x8000_0000) witness 81
+
+  method GenerateKeyPair(strength: Types.RSAStrengthBits)
+      returns (publicKey: Types.RSAPublicKey, privateKey: Types.RSAPrivateKey)
+  {
+    var pemPublic, pemPrivate := GenerateKeyPairExtern(strength);
+    privateKey := Types.RSAPrivateKey(pem := pemPrivate, strength := strength);
+    publicKey := Types.RSAPublicKey(pem := pemPublic, strength := strength);
+  }
+
+  method Decrypt(input: Types.RSADecryptInput)
+    returns (output: Result<seq<uint8>, Types.Error>)
+  {
+    :- Need(0 < |input.privateKey| && 0 < |input.cipherText|, Types.AwsCryptographicPrimitivesError( message := ""));
+    output := DecryptExtern(input.padding, input.privateKey, input.cipherText);
+  }
+
+  method Encrypt(input: Types.RSAEncryptInput)
+    returns (output: Result<seq<uint8>, Types.Error>)
+  {
+    :- Need(0 < |input.publicKey| && 0 < |input.plaintext|, Types.AwsCryptographicPrimitivesError( message := ""));
+    output := EncryptExtern(input.padding, input.publicKey, input.plaintext);
+  }
+
+  method {:extern "RSAEncryption.RSA", "GenerateKeyPairExtern"} GenerateKeyPairExtern(strength: Types.RSAStrengthBits)
+      returns (publicKey: seq<uint8>, privateKey: seq<uint8>)
+    ensures |publicKey| > 0
+    ensures |privateKey| > 0
+
+  method {:extern "RSAEncryption.RSA", "DecryptExtern"} DecryptExtern(padding: Types.RSAPaddingMode, privateKey: seq<uint8>,
+                                                                      cipherText: seq<uint8>)
+      returns (res: Result<seq<uint8>, Types.Error>)
+    requires |privateKey| > 0
+    requires |cipherText| > 0
+
+  method {:extern "RSAEncryption.RSA", "EncryptExtern"} EncryptExtern(padding: Types.RSAPaddingMode, publicKey: seq<uint8>,
+                                                                      plaintextData: seq<uint8>)
+      returns (res: Result<seq<uint8>, Types.Error>)
+    requires |publicKey| > 0
+    requires |plaintextData| > 0
+}
