AwsCryptographyPrimitives/test/TestAwsCryptographyPrimitivesHKDF.dfy
@@ -1,0 +1,117 @@
+// Copyright Amazon.com Inc. or its affiliates. All Rights Reserved.
+// SPDX-License-Identifier: Apache-2.0
+
+include "../src/Index.dfy"
+include "../src/Digest.dfy"
+
+module TestAwsCryptographyPrimitivesHKDF {
+  import Aws.Cryptography.Primitives
+  import opened Wrappers
+  import opened StandardLibrary.UInt
+  import Digest
+
+  method {:test} TestCase1() {
+    // https://tools.ietf.org/html/rfc5869#appendix-A
+    // A.1.  Test Case 1 Basic test case with SHA-256
+
+    var hash := Primitives.Types.SHA_256;
+    var IKM := [
+      11, 11, 11, 11, 11, 11, 11,
+      11, 11, 11, 11, 11, 11, 11,
+      11, 11, 11, 11, 11, 11, 11,
+      11
+    ];
+    var salt := [
+      0, 1, 2, 3,  4,  5,
+      6, 7, 8, 9, 10, 11,
+      12
+    ];
+    var info := [
+      240, 241, 242, 243,
+      244, 245, 246, 247,
+      248, 249
+    ];
+    var L := 42;
+
+    var PRK := [
+        7, 119,   9, 54,  44,  46,  50, 223,
+      13, 220,  63, 13, 196, 123, 186,  99,
+      144, 182, 199, 59, 181,  15, 156,  49,
+      34, 236, 132, 74, 215, 194, 179, 229
+    ];
+    var OKM := [
+      60, 178,  95,  37, 250, 172, 213, 122, 144,
+      67,  79, 100, 208,  54,  47,  42,  45,  45,
+      10, 144, 207,  26,  90,  76,  93, 176,  45,
+      86, 236, 196, 197, 191,  52,   0, 114,   8,
+      213, 184, 135,  24,  88, 101
+    ];
+
+    BasicExtractTest(
+      Primitives.Types.HkdfExtractInput(
+        digestAlgorithm := hash,
+        salt := Some(salt),
+        ikm := IKM
+      ),
+      PRK
+    );
+
+    BasicExpandTest(
+      Primitives.Types.HkdfExpandInput(
+        digestAlgorithm := hash,
+        prk := PRK,
+        info := info,
+        expectedLength := L
+      ),
+      OKM
+    );
+
+    BasicHkdfTest(
+      Primitives.Types.HkdfInput(
+        digestAlgorithm := hash,
+        salt := Some(salt),
+        ikm := IKM,
+        info := info,
+        expectedLength := L
+      ),
+      OKM
+    );
+  }
+
+  method BasicExtractTest(
+    input: Primitives.Types.HkdfExtractInput,
+    expectedPRK: seq<uint8>
+  )
+  {
+    var client :- expect Primitives.AtomicPrimitives();
+
+    var output :- expect client.HkdfExtract(input);
+    expect |output| == Digest.Length(input.digestAlgorithm);
+    expect output == expectedPRK;
+  }
+
+  method BasicExpandTest(
+    input: Primitives.Types.HkdfExpandInput,
+    expectedOKM: seq<uint8>
+  )
+  {
+    var client :- expect Primitives.AtomicPrimitives();
+
+    var output :- expect client.HkdfExpand(input);
+    expect |output| == input.expectedLength as nat;
+    expect output == expectedOKM;
+  }
+
+  method BasicHkdfTest(
+    input: Primitives.Types.HkdfInput,
+    expectedOKM: seq<uint8>
+  )
+  {
+    var client :- expect Primitives.AtomicPrimitives();
+
+    var output :- expect client.Hkdf(input);
+    expect |output| == input.expectedLength as nat;
+    expect output == expectedOKM;
+  }
+
+}
