AwsCryptographyPrimitives/Model/digest.smithy
@@ -1,0 +1,40 @@
+namespace aws.cryptography.primitives
+
+@enum([
+  {
+    name: "SHA_512",
+    value: "SHA_512",
+  },
+  {
+    name: "SHA_384",
+    value: "SHA_384",
+  },
+  {
+    name: "SHA_256",
+    value: "SHA_256",
+  },
+  {
+    name: "SHA_1",
+    value: "SHA_1",
+  },
+])
+string DigestAlgorithm
+
+operation Digest {
+  input: DigestInput,
+  output: DigestOutput,
+  errors: []
+}
+
+structure DigestInput {
+  @required
+  digestAlgorithm: DigestAlgorithm,
+  @required
+  message: Blob
+}
+
+@aws.polymorph#positional
+structure DigestOutput {
+  digest: Blob
+}
+
