AwsCryptographyPrimitives/Model/hkdf.smithy
@@ -1,0 +1,60 @@
+namespace aws.cryptography.primitives
+
+operation HkdfExtract {
+  input: HkdfExtractInput,
+  output: HkdfExtractOutput,
+}
+operation HkdfExpand {
+  input: HkdfExpandInput,
+  output: HkdfExpandOutput,
+}
+operation Hkdf {
+  input: HkdfInput,
+  output: HkdfOutput,
+}
+
+structure HkdfExtractInput {
+  @required
+  digestAlgorithm: DigestAlgorithm,
+  salt: Blob,
+  @required
+  ikm: Blob,
+}
+
+@aws.polymorph#positional
+structure HkdfExtractOutput {
+  prk: Blob
+}
+
+structure HkdfExpandInput {
+  @required
+  digestAlgorithm: DigestAlgorithm,
+  @required
+  prk: Blob,
+  @required
+  info: Blob,
+  @required
+  expectedLength: PositiveInteger
+}
+
+@aws.polymorph#positional
+structure HkdfExpandOutput {
+  okm: Blob,
+}
+
+structure HkdfInput {
+  @required
+  digestAlgorithm: DigestAlgorithm,
+  salt: Blob,
+  @required
+  ikm: Blob,
+  @required
+  info: Blob,
+  @required
+  expectedLength: PositiveInteger
+}
+
+@aws.polymorph#positional
+structure HkdfOutput {
+  okm: Blob,
+}
