AwsCryptographyPrimitives/Model/primitives.smithy
@@ -1,0 +1,40 @@
+namespace aws.cryptography.primitives
+
+@range(min: 0)
+integer PositiveInteger
+
+@aws.polymorph#localService(
+  sdkId: "AtomicPrimitives",
+  config: CryptoConfig,
+)
+service AwsCryptographicPrimitives {
+  version: "2020-10-24",
+  operations: [
+    GenerateRandomBytes,
+    Digest,
+    HMac,
+    HkdfExtract,
+    HkdfExpand,
+    Hkdf,
+    AESEncrypt,
+    AESDecrypt,
+    GenerateRSAKeyPair,
+    RSADecrypt,
+    RSAEncrypt,
+    GenerateECDSASignatureKey,
+    ECDSASign,
+    ECDSAVerify,
+  ],
+  errors: [AwsCryptographicPrimitivesError]
+}
+
+structure CryptoConfig {}
+
+///////////////////
+// Errors
+
+@error("client")
+structure AwsCryptographicPrimitivesError {
+  @required
+  message: String,
+}
