AwsCryptographyPrimitives/Model/random.smithy
@@ -1,0 +1,17 @@
+namespace aws.cryptography.primitives
+
+operation GenerateRandomBytes {
+  input: GenerateRandomBytesInput,
+  output: GenerateRandomBytesOutput,
+  errors: []
+}
+
+structure GenerateRandomBytesInput {
+  @required
+  length: PositiveInteger
+}
+
+@aws.polymorph#positional
+structure GenerateRandomBytesOutput {
+  data: Blob
+}
